common/ldq.lean
@@ -4,7 +4,15 @@ variables {α β : Type}
 
 open atom_type
 
-def qelim [atom_type α β] (qe : list α → fm α) (as : list α) : fm α :=
+def qe_prsv (β : Type) [atom_type α β] (qe : list α → fm α) (as : list α) : Prop := 
+  ∀ (bs : list β), ((I (qe as) bs) ↔ (∃ x, allp (val (x::bs)) as))
+
+/- 
+Requires : qe takes a list of atoms that are all dependent on 0-variable,
+  and returns formula which (1) does not contain the 0-variable, and 
+  (2) is equivalent to the conjunction of input list.
+-/
+def qelim (β) [atom_type α β] (qe : list α → fm α) (as : list α) : fm α :=
   and_o 
     (qe (@list.filter _ (dep0 β) (dec_dep0 _ _) as)) 
     (list_conj (list.map (λ (a : α), A' (decr β a)) (@list.filter _ (λ a, ¬ (dep0 β a)) 
@@ -14,6 +22,22 @@ def qelim [atom_type α β] (qe : list α → fm α) (as : list α) : fm α :=
          apply decidable.is_false (not_not_intro H)
        end) as)))
       
+      #check exp_I_list_conj
+lemma qelim_prsv [atom_type α β] {r} {qe} 
+  (hqe : ∀ as, allp (dep0 β) as → allp r as → qe_prsv β qe as)
+  {as : list α} (bs : list β) : 
+  (I (qelim β qe as) bs) ↔ (∃ b, allp (val (b::bs)) as) := 
+begin
+  apply iff.intro; intro h,
+  unfold qelim at h, 
+  rewrite exp_I_and_o at h, cases h with h1 h2,
+  rewrite hqe at h1, cases h1 with b h1, 
+  existsi b, intros a ha,
+  cases (atom_type.dec_dep0 _ β a),
+  rewrite exp_I_list_conj at h2, 
+
+end
+
 def lift_dnf_qe (β : Type) [atom_type α β] (qe : list α → fm α) : fm α → fm α 
 | (fm.true α) := ⊤'
 | (fm.false α) := ⊥'
@@ -21,7 +45,7 @@ def lift_dnf_qe (β : Type) [atom_type α β] (qe : list α → fm α) : fm α �
 | (fm.and p q) := (lift_dnf_qe p) ∧' (lift_dnf_qe q)
 | (fm.or p q) := (lift_dnf_qe p) ∨' (lift_dnf_qe q)
 | (fm.not p) := ¬' (lift_dnf_qe p) 
-| (fm.ex p) := disj (dnf (@nnf _ β _ $ lift_dnf_qe p)) (@qelim _ β _ @qe)
+| (fm.ex p) := dnf_to_fm (dnf (@nnf _ β _ $ lift_dnf_qe p)) (@qelim _ β _ @qe)
 
 lemma atoms_conj_qfree [atom_type α β] : ∀ (as : list α), qfree (list_conj (list.map (λ (a : α), A' decr β a) as )) 
 | [] := trivial
@@ -57,14 +81,10 @@ lemma ldq_qfree [atom_type α β] (qe : list α → fm α)
     apply allp_filter, apply atoms_conj_qfree 
   end
 
-def is_dnf_qe (β : Type) [atom_type α β] (qe : list α → fm α) (as : list α) : Prop := 
-  ∀ (xs : list β), ((I (qe as) xs) ↔ (∃ x, (∀ a, a ∈ as → I (A' a) (x::xs))))
-
 lemma foo (Q : list β → α → Prop) (a : α) : ∀ (bss : list (list β)), 
   list.map (λ bs, Q bs a) bss = list.map (λ (P : α → Prop), P a) (list.map Q bss)  
 | [] := eq.refl _
 | (bs::bss) := by simp 
-
 
 lemma exp_I_list_conj [atom_type α β] (xs : list β) : ∀ (ps : list (fm α)),
 I (list_conj ps) xs = all_true (list.map (λ p, I p xs) ps)  
@@ -99,6 +119,11 @@ I (list_disj ps) xs ↔ disj_list (list.map (λ p, I p xs) ps)
     apply exp_I_or_o
   end
 
+lemma exp_I_list_disj_alt [atom_type α β] (xs : list β) (ps : list (fm α)) :
+I (list_disj ps) xs ↔ some_true (list.map (λ p, I p xs) ps) := 
+iff.trans (exp_I_list_disj _ _) 
+  (by rewrite some_true_iff_disj_list) 
+
 lemma dist_ex_or (P Q : α → Prop) : (∃ x, (P x ∨ Q x)) ↔ ((∃ x, P x) ∨ (∃ x, Q x)) :=  
 begin
   apply iff.intro, intro H, cases H with x Hx, cases Hx with Hx Hx, 
@@ -124,10 +149,106 @@ lemma dist_ex_disj_list [atom_type α β] : ∀ (ps : list (β → Prop)),
     apply iff.trans, apply dist_ex_or,
     rewrite dist_ex_disj_list
   end
-  
+
+instance atom_type_to_dec_eq [atom_type α β] : decidable_eq α := atom_type.dec_eq α β 
+
+meta def ldq_prsv_core_aux := 
+`[repeat {rewrite ldq_prsv_gen}, 
+  intros a ha, 
+  apply hp, unfold atoms, 
+  apply mem_union_of_mem_right, apply ha, 
+  intros a ha, 
+  apply hp, unfold atoms, 
+  apply mem_union_of_mem_left, apply ha]
+
+lemma ldq_prsv_gen_ex [atom_type α β] 
+(qe : list α → fm α)
+(hqf : ∀ (as : list α), allp (dep0 β) as → qfree (qe as))
+(r : α → Prop)
+(hqe : ∀ (as : list α), allp (dep0 β) as → allp r as → qe_prsv β qe as)
+(p : fm α)
+(hnqf : nqfree p)
+(bs : list β)
+: some_true (list.map (λ (x : list α), I (qelim β qe x) bs) (dnf p)) ↔
+    ∃ (b : β), I p (b :: bs) := 
+begin
+  apply iff.intro; intro h,
+
+  cases h with q hq, cases hq with hq1 hq2,
+  cases (ex_arg_of_mem_map hq1) with as has,
+  cases has with has1 has2, simp at has2,
+  subst has2, rewrite qelim_prsv at hq2,
+  cases hq2 with b hb, existsi b, 
+  rewrite iff.symm dnf_prsv,
+  existsi (allp (val (b :: bs)) as),
+  apply and.intro, 
+  apply mem_map_of_mem, apply has1, 
+  apply hb, apply hnqf, apply hqe,
+
+  cases h with b hb, 
+  rewrite iff.symm dnf_prsv at hb, 
+  cases hb with q hq, cases hq with hq1 hq2,
+  cases (ex_arg_of_mem_map hq1) with as has,
+  cases has with has1 has2, subst has2, 
+  existsi (I (qelim β qe as) bs), 
+  apply and.intro, apply mem_map_of_mem,
+  apply has1, rewrite qelim_prsv, 
+  existsi b, apply hq2, apply hqe, apply hnqf
+end
+
+lemma ldq_prsv_gen [atom_type α β] (qe : list α → fm α)  
+  (hqf : ∀ as, allp (dep0 β) as → qfree (qe as)) 
+  (r : α → Prop) 
+  (hr : ∀ as, allp (dep0 β) as → allp r as → fnormal β (qe as)) 
+  (he : ∀ as, allp (dep0 β) as → allp r as → qe_prsv β qe as) : 
+  ∀ p, allp r (atoms p) → ∀ (bs : list β), I (lift_dnf_qe β qe p) bs ↔ I p bs 
+| ⊤' _ bs := iff.refl _
+| ⊥' _ bs := iff.refl _
+| (A' a) hp bs := iff.refl _
+| (p ∧' q) hp bs := 
+  begin
+    unfold lift_dnf_qe,
+    repeat {rewrite exp_I_and}, 
+    ldq_prsv_core_aux
+  end
+| (p ∨' q) hp bs := 
+  begin
+    unfold lift_dnf_qe,
+    repeat {rewrite exp_I_or}, 
+    ldq_prsv_core_aux
+  end
+| (¬' p) hp bs := 
+  begin
+    unfold lift_dnf_qe,
+    repeat {rewrite exp_I_not}, 
+    repeat {rewrite ldq_prsv_gen}, 
+    intros a ha, apply hp, apply ha
+  end
+| (∃' p) hp bs := 
+  calc 
+        I (lift_dnf_qe β qe (∃' p)) bs 
+      ↔ ∃ (b : β), I (nnf β (lift_dnf_qe β qe p)) (b :: bs) : 
+        begin
+          unfold lift_dnf_qe, unfold dnf_to_fm,
+          rewrite exp_I_list_disj_alt,
+          rewrite map_compose, apply ldq_prsv_gen_ex,
+          apply hqf, apply he, apply nnf_nqfree, 
+          apply ldq_qfree, apply hqf
+        end
+  ... ↔ I (∃' p) bs : 
+        begin
+          rewrite exp_I_ex, apply ex_iff_ex,
+          intro b, rewrite nnf_prsv,
+          rewrite ldq_prsv_gen, apply hp,
+          apply ldq_qfree, apply hqf
+        end 
+
+#exit
+
+
 lemma ldq_prsv [HA : atom_type α β] (qe : list α → fm α)  
   (H1 : ∀ (l : list α), allp (dep0 β) l → qfree (qe l))
-  (H2 : ∀ (as : list α), allp (dep0 β) as → is_dnf_qe β qe as) : 
+  (H2 : ∀ (as : list α), allp (dep0 β) as → qe_prsv β qe as) : 
     ∀ (p : fm α) (xs : list β), I (lift_dnf_qe β qe p) xs ↔ I p xs 
 | (fm.true α) xs := iff.refl _
 | (fm.false α) xs := iff.refl _
@@ -157,7 +278,7 @@ lemma ldq_prsv [HA : atom_type α β] (qe : list α → fm α)
     apply @iff.trans _ (∃ x, I (lift_dnf_qe β qe p) (x::xs)),  
     apply ex_iff_ex, 
     intro x, rewrite ldq_prsv p (x::xs), 
-    apply @iff.trans _ (∃ x, I (nnf (lift_dnf_qe β qe p)) (x::xs)),  
+    apply @iff.trans _ (∃ x, I (nnf _ (lift_dnf_qe β qe p)) (x::xs)),  
     apply ex_iff_ex, 
     intro x, rewrite nnf_prsv, 
     apply ldq_qfree, apply H1, 
@@ -166,7 +287,7 @@ lemma ldq_prsv [HA : atom_type α β] (qe : list α → fm α)
     apply (dnf_prsv _ _ (x::xs)), 
     apply nnf_nqfree, apply ldq_qfree, apply H1, 
     apply iff.trans, apply ex_iff_ex, intro b,
-    rewrite (@foo β α (λ (as : list α) (b : β), ∀ (a : α), a ∈ as → val a (b :: xs))), 
+    rewrite (@foo β α (λ (as : list α) (b : β), ∀ (a : α), a ∈ as → val (b :: xs) a)), 
     apply iff.trans, apply @dist_ex_disj_list α β _,
     unfold disj, apply iff.symm,
     apply iff.trans, apply exp_I_list_disj,
