common/atom.lean
@@ -1,0 +1,134 @@
+import .logic
+
+class atom_type (α β : Type) :=
+(val : list β → α → Prop)
+(neg : α → fm α) 
+(neg_nqfree : ∀ (a : α), nqfree (neg a))
+(neg_prsv : ∀ (a : α) (xs : list β), (interp val xs (neg a)) ↔ (interp val xs (¬' A' a)))
+(dep0 : α → Prop)
+(dec_dep0 : decidable_pred dep0)
+(decr : α → α)
+(decr_prsv : ∀ (a : α), ¬ (dep0 a) → ∀ (b : β) (bs : list β), (val bs (decr a) ↔ val (b::bs) a))
+(inh : β)
+(dec_eq : decidable_eq α)
+(normal : α → Prop)
+(normal_neg_prsv : ∀ a, normal a → allp normal (atoms (neg a)))
+(normal_decr_prsv : ∀ a, normal a → ¬ dep0 a → normal (decr a))
+
+class atom_eq_type (α β : Type) extends atom_type α β :=
+(solv0 : α → Prop)
+(dec_solv0 : decidable_pred solv0)
+(dest_solv0 : ∀ a, solv0 a → nat)
+(solv0_eq : ∀ {e : α} (He : solv0 e) {b} {bs}, val (b::bs) e
+  → list.nth_dft (atom_type.inh α β) (b::bs) (dest_solv0 e He) = b)
+(trivial : α → Prop)
+(dec_triv : decidable_pred trivial)
+(true_triv : ∀ a, trivial a → ∀ xs, val xs a)
+(subst0 : α → α → α)
+(true_subst : ∀ e, solv0 e → ∀ bs, val bs (subst0 e e))
+(subst_prsv : ∀ {e : α} (He : solv0 e), ∀ {a : α} {bs : list β}, 
+  val bs (subst0 e a) ↔ val ((list.nth_dft (atom_type.inh α β) bs (dest_solv0 e He - 1))::bs) a)
+(dest_pos : ∀ {a} {Ha : solv0 a}, ¬ trivial a → dest_solv0 a Ha > 0)
+
+-- Requires : j = 0 ↔ ¬(i = 0)
+def subst_idx : nat → nat → nat → nat 
+| 0 j 0 := j - 1
+| (i+1) _ 0 := i  
+| _ _ k := k - 1 
+
+-- Qstn : Why do I need this? (Why doesn't unfold work?)
+lemma exp_subst_idx_i0 (i) : subst_idx (i+1) 0 0 = i := 
+begin refl end
+
+variables {α β : Type}
+
+def I [atom_type α β] (p : fm α) (xs : list β) := interp (atom_type.val) xs p 
+
+lemma exp_I_and [atom_type α β] (p q : fm α) (xs : list β) : 
+  I (p ∧' q) xs = ((I p xs) ∧ (I q xs)) := eq.refl _
+
+lemma exp_I_and_o [atom_type α β] (p q : fm α) (xs : list β) : 
+  I (and_o p q) xs = ((I p xs) ∧ (I q xs)) := 
+begin
+  apply (cases_and_o' (λ p q pq, ((I pq xs) = ((I p xs) ∧ (I q xs)))) p q), 
+  repeat {unfold I, unfold interp, simp},
+  unfold I, unfold interp 
+end
+
+lemma exp_I_or [atom_type α β] (p q : fm α) (xs : list β) : 
+  I (p ∨' q) xs = ((I p xs) ∨ (I q xs)) := eq.refl _
+
+lemma exp_I_or_o [atom_type α β] (p q : fm α) (xs : list β) : 
+  I (or_o p q) xs ↔ ((I p xs) ∨ (I q xs)) := 
+begin
+  apply (cases_or_o' (λ p q pq, ((I pq xs) ↔ ((I p xs) ∨ (I q xs)))) p q), 
+  repeat {unfold I, unfold interp, simp},
+  unfold I, unfold interp 
+end
+
+lemma exp_I_not [atom_type α β] (p : fm α) (xs : list β) : 
+  I (¬' p) xs = ¬ (I p xs) := eq.refl _
+
+lemma exp_I_not_o [atom_type α β] (p : fm α) :
+  ∀ (xs : list β), I (not_o p) xs ↔ ¬ (I p xs) :=
+by cases p; {unfold not_o, unfold I, unfold interp, try {simp}}
+
+lemma exp_I_ex [atom_type α β] (p : fm α) (xs) : @I α β _ (∃' p) xs = ∃ x, (I p (x::xs)) := 
+by unfold I; unfold interp
+
+lemma exp_I_top [atom_type α β] (xs) : @I α β _ ⊤' xs = true := 
+by unfold I; unfold interp
+
+lemma exp_I_bot [atom_type α β] (xs) : @I α β _ ⊥' xs = false := 
+by unfold I; unfold interp
+
+def fnormal_alt (β) [atom_type α β] (p : fm α) := 
+  allp (atom_type.normal β) (@atoms _ (atom_type.dec_eq _ β) p)
+
+def fnormal (β) [atom_type α β] : fm α → Prop 
+| ⊤' := true
+| ⊥' := true
+| (A' a) := atom_type.normal β a 
+| (p ∧' q) := fnormal p ∧ fnormal q
+| (p ∨' q) := fnormal p ∧ fnormal q
+| (¬' p) := fnormal p
+| (∃' p) := fnormal p
+
+lemma fnormal_iff_fnormal_alt [atom_type α β] : 
+  ∀ {p : fm α}, fnormal β p ↔ fnormal_alt β p 
+| ⊤' := true_iff_true trivial (λ a ha, by cases ha)
+| ⊥' := true_iff_true trivial (λ a ha, by cases ha)
+| (A' a) := 
+  begin 
+    unfold fnormal, 
+    unfold fnormal_alt, unfold atoms,
+    apply iff.intro; intro h, 
+    intros a' ha', cases ha' with he he,
+    subst he, apply h, cases he, 
+    apply h, apply or.inl rfl
+  end
+| (p ∧' q) := 
+  begin 
+    unfold fnormal, 
+    repeat {rewrite fnormal_iff_fnormal_alt}, 
+    apply iff.symm, apply exp_allp_union
+  end
+| (p ∨' q) := 
+  begin 
+    unfold fnormal, 
+    repeat {rewrite fnormal_iff_fnormal_alt}, 
+    apply iff.symm, apply exp_allp_union
+  end
+| (¬' p) := 
+  begin 
+    unfold fnormal, 
+    rewrite fnormal_iff_fnormal_alt, refl
+  end
+| (∃' p) := 
+  begin 
+    unfold fnormal, 
+    rewrite fnormal_iff_fnormal_alt, refl
+  end
+
+def disj_to_prop (β) [atom_type α β] (as : list α) (bs : list β) : Prop :=
+  allp (atom_type.val bs) as
