common/lnq.lean
@@ -1,0 +1,101 @@
+import .nnf .predicates
+
+variables {α β : Type}
+
+def lift_nnf_qe (β) [Hα : atom_type α β] (qe : fm α → fm α) : fm α → fm α 
+| (p ∧' q) := and_o (lift_nnf_qe p) (lift_nnf_qe q)
+| (p ∨' q) := or_o  (lift_nnf_qe p) (lift_nnf_qe q)
+| (¬' p) := not_o (lift_nnf_qe p)
+| (∃' p) := qe (@nnf α β Hα (lift_nnf_qe p))
+| p := p
+
+lemma and_o_prsv_qfree (p q : fm α) : 
+  qfree p → qfree q → qfree (and_o p q) := 
+λ Hp Hq, 
+  begin 
+    cases p; cases q; 
+    {trivial <|> apply Hp <|> apply Hq <|> {apply (and.intro Hp Hq)}}
+  end
+
+lemma or_o_prsv_qfree (p q : fm α) : 
+  qfree p → qfree q → qfree (or_o p q) := 
+λ Hp Hq, 
+  begin 
+    cases p; cases q; 
+    {trivial <|> apply Hp <|> apply Hq <|> {apply (and.intro Hp Hq)}}
+  end
+
+lemma not_o_prsv_qfree (p : fm α) (H : qfree p) : qfree (not_o p) := 
+begin cases p; {trivial <|> apply H} end
+
+lemma lnq_qfree [Hα : atom_type α β] (qe : fm α → fm α) 
+(H : ∀ (f : fm α), nqfree f → qfree (qe f)) : 
+  ∀ (f : fm α), qfree (@lift_nnf_qe α β Hα qe f) :=
+λ f, fm.rec_on f trivial trivial 
+  (λ a, trivial)
+  (λ f1 f2 H1 H2, and_o_prsv_qfree _ _ H1 H2)
+  (λ f1 f2 H1 H2, or_o_prsv_qfree _ _ H1 H2)
+  (λ f1 H1, not_o_prsv_qfree _ H1)
+  (λ f1 H1, begin apply H, apply nnf_nqfree, apply H1 end)
+
+open tactic
+
+lemma lnq_prsv_gen 
+  [Hα : atom_type α β] (qe : fm α → fm α) 
+  (hqe : qfree_prsv qe) 
+  (r : fm α → Prop) 
+  (hdc : down_closed r)
+  (hqc : closed qe r)
+  (hnc : closed (nnf β) r)
+  (hlc : ∀ f, closed f r → closed (lift_nnf_qe β f) r)
+  (hi : ∀ (p : fm α), nqfree p → r p → ∀ (xs : list β), I (qe p) xs ↔ ∃ x, I p (x::xs)) : 
+  ∀ (p : fm α), r p → ∀ (xs : list β), I (lift_nnf_qe β qe p) xs ↔ I p xs 
+| ⊤' _ bs := iff.refl _
+| ⊥' _ bs := iff.refl _
+| (A' a) _ bs := iff.refl _
+| (p ∧' q) hr xs := 
+  begin 
+    unfold lift_nnf_qe, rewrite exp_I_and, 
+    rewrite exp_I_and_o, 
+    repeat {rewrite lnq_prsv_gen}, 
+    apply hdc _ _ (down.andr _ _) hr, 
+    apply hdc _ _ (down.andl _ _) hr 
+  end 
+| (p ∨' q) hr xs := 
+  begin 
+    unfold lift_nnf_qe, rewrite exp_I_or, 
+    rewrite exp_I_or_o, repeat {rewrite lnq_prsv_gen},
+    apply hdc _ _ (down.orr _ _) hr, 
+    apply hdc _ _ (down.orl _ _) hr 
+  end 
+| (¬' p) hr xs := 
+  begin 
+    unfold lift_nnf_qe, rewrite exp_I_not,  
+    rewrite exp_I_not_o, repeat {rewrite lnq_prsv_gen},
+    apply hdc _ _ (down.not _) hr 
+  end
+| (∃' p) hr xs := 
+  begin 
+    unfold lift_nnf_qe, rewrite exp_I_ex,
+    rewrite hi, apply ex_iff_ex, intro b, 
+    rewrite nnf_prsv, apply lnq_prsv_gen, 
+    apply hdc _ _ (down.ex _) hr, 
+    apply lnq_qfree, apply hqe, 
+    apply nnf_nqfree, apply lnq_qfree,
+    apply hqe, apply hnc, apply hlc, apply hqc, 
+    apply hdc _ _ (down.ex _) hr 
+  end
+
+lemma lnq_prsv [Hα : atom_type α β] (qe : fm α → fm α) 
+  (hqe : qfree_prsv qe) 
+  (hi : ∀ (p : fm α), nqfree p → ∀ (xs : list β), I (qe p) xs ↔ ∃ x, I p (x::xs)) : 
+  ∀ (p : fm α) (xs : list β), I (lift_nnf_qe β qe p) xs ↔ I p xs :=
+begin
+  intro p, apply (lnq_prsv_gen _ _ (λ _, true)),
+  intros _ _ _ _, trivial, 
+  intros _ _,  trivial, 
+  intros _ _,  trivial, 
+  intros _ _ _ _, trivial, 
+  intros q hf h', apply hi, 
+  apply hf, trivial, apply hqe
+end
