common/predicates.lean
@@ -1,0 +1,29 @@
+import .atom
+
+variables {α β : Type}
+
+def qfree_prsv (qe : fm α → fm α) := 
+∀ (p : fm α), nqfree p → qfree (qe p)
+
+def normal_prsv (β) [atom_type α β] (qe : fm α → fm α) := 
+∀ (p : fm α), nqfree p → fnormal β p → qfree (qe p)
+
+def interp_prsv_ex (β) [atom_type α β] (qe : fm α → fm α) (p) := 
+∀ (bs : list β), I (qe p) bs = ∃ b, (I p (b::bs))
+
+def interp_prsv (β) [atom_type α β] (qe : fm α → fm α) (p) := 
+∀ (bs : list β), I (qe p) bs = I p bs
+
+inductive down : fm α → fm α → Prop 
+| andl : ∀ p q, down (p ∧' q) p
+| andr : ∀ p q, down (p ∧' q) q
+| orl  : ∀ p q, down (p ∨' q) p
+| orr  : ∀ p q, down (p ∨' q) q
+| not  : ∀ p, down (¬' p) p
+| ex   : ∀ p, down (∃' p) p
+
+def down_closed (r : fm α → Prop) : Prop := 
+∀ (p q : fm α), down p q → r p → r q
+
+def closed (f : α → α) (r : α → Prop) : Prop := 
+∀ a, r a → r (f a)
