presburger/correctness.lean
@@ -1,0 +1,116 @@
+import .atom ..common.lnq ..common.ldq ..common.predicates 
+
+variables {α β : Type}
+
+namespace pbgr
+
+lemma fnormal_down_closed : @down_closed (pbgr.atom) (fnormal int)  
+| ⊤' _ hd _ := by cases hd
+| ⊥' _ hd _ := by cases hd
+| (A' a) _ hd _ := by cases hd
+| (p ∧' q) r hd hn := 
+  by {unfold fnormal at hn, cases hn, cases hd; assumption}
+| (p ∨' q) r hd hn := 
+  by {unfold fnormal at hn, cases hn, cases hd; assumption}
+| (¬' p) r hd hn := by {cases hd, apply hn}
+| (∃' p) r hd hn := by {cases hd, apply hn}
+
+meta def nnf_closed_fnormal_aux := 
+`[unfold nnf, unfold fnormal,
+  unfold fnormal at hn, cases hn with hnp hnq, 
+  cases (nnf_closed_fnormal_core hnp) with hnp1 hnp2,
+  cases (nnf_closed_fnormal_core hnq) with hnq1 hnq2,
+  apply and.intro; apply and.intro; assumption]
+
+lemma nnf_closed_fnormal_core : ∀ {p : fm pbgr.atom}, 
+  fnormal int p → fnormal int (nnf int p) ∧ fnormal int (nnf int (¬' p))
+| ⊤' hn := and.intro trivial trivial 
+| ⊥' hn := and.intro trivial trivial 
+| (A' a) hn := 
+  begin
+    unfold nnf, apply and.intro, 
+    apply hn, rewrite fnormal_iff_fnormal_alt,
+    apply atom_type.normal_neg_prsv, apply hn
+  end
+| (p ∧' q) hn := by nnf_closed_fnormal_aux
+| (p ∨' q) hn := by nnf_closed_fnormal_aux
+| (¬' p) hn := 
+  begin
+    apply and.symm, unfold fnormal at hn,
+    unfold nnf, apply nnf_closed_fnormal_core hn
+  end
+| (∃' p) hn := 
+  begin unfold nnf, apply and.intro; trivial end
+
+lemma nnf_closed_fnormal : closed (@nnf pbgr.atom int _) (fnormal int) := 
+λ p hn, (nnf_closed_fnormal_core hn)^.elim_left
+
+lemma atoms_and_o_subset {p q : fm pbgr.atom} : 
+  atoms (and_o p q) ⊆ atoms p ∪ atoms q := 
+begin
+  apply cases_and_o' (λ p' q' r, atoms r ⊆ atoms p' ∪ atoms q') p q;
+  intros a ha, 
+  apply mem_union_of_mem_right ha, 
+  apply mem_union_of_mem_left ha, 
+  apply mem_union_of_mem_left ha, 
+  apply mem_union_of_mem_right ha, 
+  apply ha
+end
+
+lemma lnq_closed_fnormal (f : fm atom → fm atom) 
+ (hc : closed f (fnormal ℤ)) : closed (lift_nnf_qe ℤ f) (fnormal ℤ) 
+| ⊤' hn := trivial
+| ⊥' hn := trivial
+| (A' a) hn := by {unfold lift_nnf_qe, apply hn}
+| (p ∧' q) hn := 
+  begin
+    unfold fnormal at hn , cases hn with hnp hnq,
+    unfold lift_nnf_qe, apply cases_and_o, trivial, 
+    apply lnq_closed_fnormal, apply hnp,
+    apply lnq_closed_fnormal, apply hnq,
+    apply and.intro; apply lnq_closed_fnormal; assumption, 
+  end
+| (p ∨' q) hn := 
+  begin
+    unfold fnormal at hn , cases hn with hnp hnq,
+    unfold lift_nnf_qe, apply cases_or_o, trivial, 
+    apply lnq_closed_fnormal, apply hnp,
+    apply lnq_closed_fnormal, apply hnq,
+    apply and.intro; apply lnq_closed_fnormal; assumption, 
+  end
+| (¬' p) hn := 
+  begin
+    unfold fnormal at hn, unfold lift_nnf_qe, apply cases_not_o, 
+    trivial, trivial, apply lnq_closed_fnormal, apply hn
+  end
+| (∃' p) hn := 
+  begin
+    unfold lift_nnf_qe, apply hc, 
+    apply nnf_closed_fnormal, 
+    apply lnq_closed_fnormal, apply hn
+  end
+
+theorem lnq_prsv 
+  (qe : fm pbgr.atom → fm pbgr.atom) 
+  (hqe : closed qe (fnormal int))
+  (hqf : qfree_prsv qe) (hn : normal_prsv int qe) 
+  (hi : ∀ p, nqfree p → fnormal int p → ∀ (bs : list int), I (qe p) bs ↔ ∃ b, (I p (b::bs))) : 
+∀ p, fnormal int p → ∀ (bs : list int), I (lift_nnf_qe int qe p) bs ↔ I p bs :=
+@lnq_prsv_gen pbgr.atom int pbgr.atom_type 
+  qe hqf (fnormal int) fnormal_down_closed hqe 
+  nnf_closed_fnormal lnq_closed_fnormal hi 
+
+theorem ldq_prsv 
+  (qe : list pbgr.atom → fm pbgr.atom) 
+  (hqf : ∀ as, allp dep0 as → qfree (qe as)) 
+  (hn : ∀ as, allp dep0 as → allp normal as → fnormal int (qe as)) 
+  (he : ∀ as, allp dep0 as → allp normal as → is_dnf_qe int qe as) :
+  ∀ p, fnormal int p → ∀ (bs : list int), I (lift_dnf_qe int qe p) bs ↔ I p bs :=
+
+  
+sorry 
+
+
+end pbgr
+
+
